Regex/Regular.lean
@@ -27,240 +27,99 @@ variable {s : Pos w} {cap : Captures w} {t : IccFrom s} {a : IccTo s} {b : IccFr
 like captures -/
 def MatchPartialFree (r : Regex α) :=
   ∀ {w : List α} {s : Pos w} {cap : Captures w}
-      {term : r.Terminates w s cap} {t : Pos w},
-      t ∈ (r.matchPartial w s cap term).map Prod.fst →
-    ∀ (wa : List α) (wb : List α) (cap₁ : Captures (wa ++ w.extract s.val t.val ++ wb))
-      (term₁ : r.Terminates (wa ++ w.extract s.val t.val ++ wb) (s.recycle t wa wb).1 cap₁),
-    (s.recycle t wa wb).2 ∈
-      (r.matchPartial (wa ++ w.extract s.val t.val ++ wb)
-        (s.recycle t wa wb).1 cap₁ term₁).map Prod.fst
+      {term : r.Terminates w s cap} {s' : Pos w} {cap' : Captures w}
+      (mem : (s', cap') ∈ r.matchPartial w s cap term)
+      (wa : List α) (wb : List α) (cap₁ : Captures (wa ++ w.extract s.val s'.val ++ wb))
+      (term₁ : r.Terminates (wa ++ w.extract s.val s'.val ++ wb)
+        (s.recycle s s' (monotone mem) wa wb) cap₁),
+    ∃ cap₁', (s'.recycle s s' (le_refl _) wa wb, cap₁') ∈
+      r.matchPartial (wa ++ w.extract s.val s'.val ++ wb)
+        (s.recycle s s' (monotone mem) wa wb) cap₁ term₁
 
 theorem matchPartialFree_bot : MatchPartialFree ([/⊥/] : Regex α) := by
   simp [MatchPartialFree, matchPartial_bot]
 
 theorem matchPartialFree_empty : MatchPartialFree ([//] : Regex α) := by
-  simp only [MatchPartialFree, matchPartial_empty, List.map_cons, List.map_nil, List.mem_cons,
-    ← Icc.val_inj, List.not_mem_nil, or_false, List.extract_eq_drop_take, Icc.recycle_snd_val,
-    Icc.recycle_fst_val, Nat.add_eq_left]
-  intro w s cap term t teq
+  simp only [MatchPartialFree, matchPartial_empty, List.mem_cons, Prod.mk.injEq, ← Icc.val_inj,
+    List.not_mem_nil, or_false, List.extract_eq_drop_take, Icc.recycle_val, tsub_self, add_zero,
+    Nat.add_eq_left, exists_eq_right, forall_and_index]
+  intro w s cap term t cap' teq
   simp [teq]
 
 theorem matchPartialFree_unit (c : α) : MatchPartialFree [/c/] := by
-  simp only [MatchPartialFree, matchPartial_unit, List.mem_map, List.mem_dite_nil_right,
-    List.mem_cons, List.not_mem_nil, or_false, ← Icc.val_inj, Prod.exists, Prod.mk.injEq,
-    Icc.succOfIndex_val, exists_and_left, exists_prop, exists_and_right, ↓existsAndEq, and_true,
-    List.extract_eq_drop_take, List.append_assoc, Icc.recycle_fst_val, Icc.recycle_snd_val,
-    forall_exists_index, and_imp]
-  intro w s cap term t s' s'add wsc s't wa wb cap₁ term₁
+  simp only [MatchPartialFree, matchPartial_unit, List.mem_dite_nil_right, List.mem_cons,
+    Prod.mk.injEq, ← Icc.val_inj, Icc.succOfIndex_val, List.not_mem_nil, or_false, exists_and_left,
+    exists_prop, List.extract_eq_drop_take, List.append_assoc, Icc.recycle_val, tsub_self, add_zero,
+    Nat.add_left_cancel_iff, ↓existsAndEq, and_true, forall_and_index]
+  intro w s cap term s' cap' s'add wsc capeq wa wb cap₁ term₁
   have ⟨lt, wsc⟩ := List.getElem?_eq_some_iff.mp wsc
   have one : 1 ≤ w.length - s.val := by
     by_contra!
     rw [Nat.lt_one_iff, Nat.sub_eq_zero_iff_le] at this
     exact not_le.mpr lt this
-  use ⟨wa.length + 1, by simp [← s't, s'add, min_eq_left_iff.mpr one]⟩
   suffices (if s.val < w.length then w[s.val]? else wb[0]?) = some c by
-    simpa [← s't, s'add, List.getElem?_append]
+    simpa [s'add, List.getElem?_append]
   rw [Nat.le_sub_iff_add_le' s.is_le, ← Nat.lt_iff_add_one_le] at one
   simp [one, wsc]
 
-theorem matchPartialFree_concat (q r : Regex α) (qf : q.MatchPartialFree)
+theorem matchPartialFree_concat {q r : Regex α} (qf : q.MatchPartialFree)
     (rf : r.MatchPartialFree)
     : [/⟨q⟩ ⟨r⟩/].MatchPartialFree := by
-  simp? [MatchPartialFree, matchPartial_concat] at qf rf ⊢
-  --intro w s cap term t mem wa wb cap₁ term₁
-  --rcases mem with ⟨mat, qmem, rmem⟩
+  simp only [MatchPartialFree, matchPartial_concat, List.mem_flatten, List.mem_pmap, Prod.exists,
+    ↓existsAndEq, true_and, forall_exists_index] at ⊢
+  intro w s cap term s'' cap'' s' cap' qmem rmem wa wb cap₁ term₁
+  -- Please excuse the massive ▸ spam ahead
+  have eaear := List.extract_append_extract_assoc_right (monotone qmem) (monotone rmem) wa wb
+  have rear := Icc.recycle_extract_append_right (le_refl s) (monotone qmem) (monotone rmem) wa wb
+  have eaeal := List.extract_append_extract_assoc_left (monotone qmem) (monotone rmem) wa wb
+  have real := Icc.recycle_extract_append_left (monotone qmem) (monotone rmem) (le_refl s'') wa wb
+  -- And the ▸s have gotten slow
+  have qf₁ := qf qmem wa (w.extract s'.val s''.val ++ wb)
+  simp only [rear] at qf₁
+  rw! (castMode := .all) [eaear] at qf₁
+  specialize qf₁ cap₁ (concat_terminates.mp term₁).1
+  have ⟨cap₁', qf₁⟩ := qf₁
+  simp only at qf₁
+  have rf₁ := rf rmem (wa ++ w.extract s.val s'.val) wb
+  simp only [real] at rf₁
+  rw! (castMode := .all) [eaeal] at rf₁
+  specialize rf₁ cap₁' (by
+    have term' := (concat_terminates.mp term₁).2 _ qf₁
+    simp only at term'
+    refine cast ?_ term'
+    congr 1
+    rw [Icc.recycle_extract_append_right (monotone qmem) (le_refl _),
+      Icc.recycle_extract_append_left (monotone qmem) (le_refl _)]
+    · simp only [List.extract_eq_drop_take, eqRec_eq_cast, cast_cast, cast_eq]
+    exact monotone rmem)
+  have ⟨cap₁'', rf₁⟩ := rf₁
+  simp only at rf₁
+  refine ⟨cap₁'', _, _, qf₁, cast ?_ rf₁⟩
+  congr 2
+  rw [Icc.recycle_extract_append_right (monotone qmem) (le_refl _),
+    Icc.recycle_extract_append_left (monotone qmem) (le_refl _)]
+  · simp only [List.extract_eq_drop_take, eqRec_eq_cast, cast_cast, cast_eq]
+  exact (monotone rmem)
 
-theorem exists_congr' {α β : Type*} {p : α → Prop} {q : β → Prop} (f : α → β)
-    : (∀ a : α, p a ↔ q (f a)) → (∀ b : β, (∀ a : α, f a ≠ b) → ¬q b) →
-      ((∃ a : α, p a) ↔ ∃ b : β, q b) := by
-  intro alla noa
-  constructor
-  · rintro ⟨a, ha⟩
-    exact ⟨f a, (alla a).mp ha⟩
-  · rintro ⟨b, hb⟩
-    specialize noa b
-    rw [imp_not_comm] at noa
-    push_neg at noa
-    obtain ⟨a, ha⟩ := noa hb
-    exact ⟨a, (alla a).mpr (ha ▸ hb)⟩
+theorem matchPartialFree_or {q r : Regex α} (qf : q.MatchPartialFree)
+    (rf : r.MatchPartialFree)
+    : [/⟨q⟩ | ⟨r⟩/].MatchPartialFree := by
+  simp only [MatchPartialFree, matchPartial_or, List.mem_append]
+  intro w s cap term s' cap' mem wa wb cap₁ term₁
+  rcases mem with mem | mem
+  · have ⟨cap₁', mem'⟩ := qf mem wa wb cap₁ (or_terminates.mp term₁).1
+    exact ⟨cap₁', Or.inl mem'⟩
+  · have ⟨cap₁', mem'⟩ := rf mem wa wb cap₁ (or_terminates.mp term₁).2
+    exact ⟨cap₁', Or.inr mem'⟩
 
-theorem matchPartial_subst {s sₑ : Pos w} {cap : Captures w} {t : IccFrom s}
-    {cap' : Captures w} (hs : s = sₑ)
-    : ((t, cap') ∈ r.matchPartial w s cap) =
-      ((⟨t.val, hs ▸ t.property⟩, cap') ∈ r.matchPartial w sₑ cap) := by
-  congr
-  rw [Subtype.heq_iff_coe_eq]
-  simp [hs]
-
-omit deq in
-theorem iccFrom_extract_fst_le (s' : IccFrom (s.extract t a b).fst)
-    : s.val ≤ s'.val + a.val ∧ s'.val + a.val ≤ b.val := by
-  have ab : a.val ≤ b.val := .trans a.is_le <| .trans t.is_ge b.is_ge
-  constructor
-  · have s'ge := s'.is_ge
-    simp only [List.extract_eq_drop_take, Icc.extract_fst_val, tsub_le_iff_right] at s'ge
-    exact s'ge
-  · have s'le := s'.is_le
-    simp only [List.length_extract_nat' ab, b.is_le] at s'le
-    rw [Nat.le_sub_iff_add_le ab] at s'le
-    exact s'le
-
-omit deq in
-theorem iccFrom_extract_fst_le_length (s' : IccFrom (s.extract t a b).fst)
-    : s.val ≤ s'.val + a.val ∧ s'.val + a.val ≤ w.length := by
-  obtain ⟨lt, rt⟩ := iccFrom_extract_fst_le s'
-  exact ⟨lt, .trans rt b.is_le⟩
-
-omit deq in
-theorem iccFrom_extract_fst_le_length' (s' : IccFrom (s.extract t a b).fst)
-    : 0 ≤ s'.val + a.val ∧ s'.val + a.val ≤ w.length := by
-  obtain ⟨lt, rt⟩ := iccFrom_extract_fst_le s'
-  exact ⟨.trans (Nat.zero_le _) lt, .trans rt b.is_le⟩
-
-omit deq in
-theorem icc_extract_le_sub (a : IccTo s) (b : IccFrom t) {s' : IccFrom s}
-    (hs' : s'.val ≤ b.val)
-    : (s.extract t a b).fst.val ≤ s'.val - a.val ∧
-      s'.val - a.val ≤ (w.extract a.val b.val).length := by
-  simp only [List.extract_eq_drop_take, Icc.extract_fst_val, tsub_le_iff_right,
-    List.length_take, List.length_drop, le_inf_iff]
-  rw [Nat.sub_add_cancel (.trans a.is_le s'.is_ge)]
-  rw [Nat.sub_add_cancel (.trans a.is_le <| .trans t.is_ge b.is_ge),
-    Nat.sub_add_cancel (.trans a.is_le s.is_le)]
-  exact ⟨s'.is_ge, hs', s'.is_le⟩
-
-omit deq in
-theorem icc_extract_ne {sₑ' : IccFrom (s.extract t a b).fst}
-    {sₑ''' : IccFrom (s.extract t a b).fst} (hsₑ : sₑ'''.val < sₑ'.val)
-    : (∀ sₑ'' : IccFrom sₑ', sₑ'''.val ≠ sₑ''.val) ∧
-      (∀ s'' : IccFrom (⟨sₑ'.val + a.val, iccFrom_extract_fst_le_length sₑ'⟩ : IccFrom s),
-        sₑ'''.val + a.val ≠ s''.val) := by
-  have ne := (fun sₑ'' : IccFrom sₑ' ↦ Icc.ne_of_lt_of_mem_iccFrom sₑ'' hsₑ)
-  refine ⟨ne, ?_⟩
-  intro s''
-  contrapose! ne
-  refine ⟨⟨s''.val - a.val, ?_⟩, ?_⟩
-  · have sₑ'''le := ne ▸ iccFrom_extract_fst_le sₑ'''
-    constructor
-    · exact Nat.le_sub_of_add_le s''.is_ge
-    · simp only [List.length_extract_nat' (.trans a.is_le <| .trans t.is_ge b.is_ge) b.is_le]
-      rw [Nat.sub_le_sub_iff_right (.trans a.is_le <| .trans t.is_ge b.is_ge)]
-      exact sₑ'''le.right
-  simp only []
-  exact Nat.eq_sub_of_add_eq ne
-
-theorem matchPartialIsMatch_concat (q r : Regex α)
-    : matchPartialShrink q → matchPartialShrink r → matchPartialShrink (concat q r) := by
-  intro qm rm
-  simp only [matchPartialShrink, matchPartial,
-    Icc.iccFrom_expandZero, List.pure_def, List.bind_eq_flatMap, List.mem_map,
-    List.mem_flatMap, List.mem_cons, List.not_mem_nil, or_false, Prod.exists,
-    ← Icc.val_inj, Prod.mk.injEq, Icc.widenLeft_val, exists_eq_right_right',
-    exists_and_right, Icc.extract_fst_val, Icc.extract_snd_val]
-  intro w s cap t a b capₑ
-  simp only [matchPartialShrink, List.mem_map, Prod.exists,
-    exists_and_right, exists_eq_right] at qm rm
-  symm
-  have ab : a.val ≤ b.val := .trans a.is_le <| .trans t.is_ge b.is_ge
-  apply exists_congr' (fun s' ↦ ⟨s'.val + a.val, iccFrom_extract_fst_le_length s'⟩)
-  rotate_right 1
-  · push_neg
-    rintro s''' nos''' ⟨cap'', s', cap', memq, s'', memr, s'''s''⟩
-    contrapose! nos'''
-    symm at s'''s''
-    refine ⟨⟨s'''.val - a.val, icc_extract_le_sub a b (trans nos''' b.is_ge)⟩, ?_⟩
-    simp only [← Icc.val_inj]
-    rw [Nat.sub_add_cancel (.trans a.is_le <| .trans s'.is_ge <| trans s''.is_ge s'''s'')]
-  intro sₑ'''
-  refine and_congr ?_ ?_; rotate_left 1
-  · simp only []
-    rw [eq_tsub_iff_add_eq_of_le (.trans a.is_le t.is_ge)]
-  rw [exists_comm]
-  conv_rhs => rw [exists_comm]
-  apply exists_congr' (fun s₂' ↦ ⟨s₂'.val + a.val, iccFrom_extract_fst_le_length s₂'⟩)
-  rotate_right 1
-  · push_neg
-    intro s' nos' cap'' cap' memq s'' rmem
-    contrapose! nos'
-    refine ⟨⟨s'.val - a.val, icc_extract_le_sub a b ?_⟩, by
-      simp only [← Icc.val_inj]
-      rw [Nat.sub_add_cancel (.trans a.is_le s'.is_ge)]⟩
-    obtain ⟨sₑ'''ge, sₑ'''le⟩ := iccFrom_extract_fst_le sₑ'''
-    simp only [Icc.extract_fst_val] at nos'
-    exact .trans s''.is_ge <| trans (symm nos') sₑ'''le
-  intro sₑ'
-  let s' : IccFrom s := ⟨sₑ'.val + a.val, iccFrom_extract_fst_le_length sₑ'⟩
-  by_cases! sₑlt : sₑ'''.val < sₑ'.val
-  · obtain ⟨ne, ne'⟩ := icc_extract_ne sₑlt
-    simp [ne, ne']
-  let s''' : IccFrom (s'.expandZero) := ⟨sₑ'''.val + a.val, by
-    have le := iccFrom_extract_fst_le_length sₑ'''
-    simp only [Icc.expandZero_val, s']
-    exact ⟨Nat.add_le_add_right sₑlt a.val, le.right⟩⟩
-  let a' : IccTo (s'.expandZero) := ⟨a.val, ⟨Nat.zero_le _, .trans a.is_le s'.is_ge⟩⟩
-  let b' : IccFrom s' := ⟨b.val, ⟨(iccFrom_extract_fst_le sₑ').right, b.is_le⟩⟩
-  let b'' : IccFrom s''' := ⟨b.val, ⟨(iccFrom_extract_fst_le sₑ''').right, b.is_le⟩⟩
-  specialize qm w s cap s' a b' capₑ
-  specialize rm w s'.expandZero
-  rw [forall_comm] at rm; specialize rm s'''
-  rw [forall_comm] at rm; specialize rm a'
-  rw [forall_comm] at rm; specialize rm b''
-  simp only [Icc.extract_fst_val, Icc.iccFrom_expandZero, s', b', a', s''', b''] at qm rm
-  rw [iff_comm]
-  have exeq := s.extract_fst_eq t s' a b b'.is_ge
-  simp only [s'] at exeq
-  simp only [matchPartial_subst (Eq.symm exeq), Icc.extract_fst_val, Icc.extract_snd_val,
-    add_tsub_cancel_right, Subtype.coe_eta] at qm
-  have exeq' : (s'.expandZero.extract s''' a' b'').fst = sₑ'.expandZero := by
-    simp [← Icc.val_inj, s', a']
-  simp only [Icc.extract_fst_val, s', a', s''', b''] at exeq'
-  simp only [Icc.extract_fst_val, matchPartial_subst exeq', Icc.iccFrom_expandZero,
-    Icc.extract_snd_val, add_tsub_cancel_right] at rm
-  constructor
-  · rintro ⟨cap'', cap', memq, s'', memr, s'''s''⟩
-    obtain ⟨capₑ', memqₑ⟩ := qm.mp ⟨cap', memq⟩
-    have s'''s'' : (s''' : IccFrom s') = s'' := by simp [← Icc.val_inj, ← s'''s'', s''']
-    simp only [s'''] at s'''s''
-    obtain ⟨capₑ'', memrₑ⟩ := (rm cap' capₑ').mp ⟨cap'', s'''s'' ▸ memr⟩
-    use capₑ'', capₑ', memqₑ, ?_
-  · rintro ⟨capₑ'', capₑ', memqₑ, sₑ'', memrₑ, s'''s''⟩
-    obtain ⟨cap', memq⟩ := qm.mpr ⟨capₑ', memqₑ⟩
-    simp only [s'''s'', Subtype.coe_eta] at rm
-    obtain ⟨cap'', memr⟩ := (rm cap' capₑ').mpr ⟨capₑ'', memrₑ⟩
-    refine ⟨cap'', cap', memq, s''', ?_⟩
-    simp only [Icc.extract_fst_val, s'''s'', and_true, s''']
-    exact memr
-
-theorem matchPartialIsMatch_or (q r : Regex α)
-    : matchPartialShrink q → matchPartialShrink r → matchPartialShrink (or q r) := by
-  intro qm rm
-  simp only [matchPartialShrink, matchPartial, List.map_append, List.mem_append,
-    List.mem_map, ← Icc.val_inj, Prod.exists, exists_and_right, Icc.extract_fst_val,
-    Icc.extract_snd_val]
-  intro w s cap t a b capₑ
-  simp only [matchPartialShrink, List.mem_map, Prod.exists,
-    exists_and_right, exists_eq_right] at qm rm
-  specialize qm w s cap t a b capₑ
-  specialize rm w s cap t a b capₑ
-  constructor
-  · intro or
-    rcases or with ⟨s', ⟨cap', mem⟩, s't⟩ | ⟨s', ⟨cap', mem⟩, s't⟩
-    case' mp.inl => left
-    case' mp.inr => right; revert qm rm; intro rm qm
-    case mp.inl | mp.inr =>
-      simp only [show s' = t by simp [← Icc.val_inj, s't]] at mem
-      obtain ⟨capₑ', memₑ⟩ := qm.mp ⟨cap', mem⟩
-      refine ⟨⟨t.val - a.val, icc_extract_le_sub a b b.is_ge⟩,
-        ⟨capₑ', memₑ⟩, by simp⟩
-  · intro or
-    rcases or with ⟨sₑ', ⟨capₑ', memₑ⟩, s't⟩ | ⟨sₑ', ⟨capₑ', memₑ⟩, s't⟩
-    case' mpr.inl => left
-    case' mpr.inr => right; revert qm rm; intro rm qm
-    case mpr.inl | mpr.inr =>
-      simp only [show sₑ' = ⟨t.val - a.val, icc_extract_le_sub a b b.is_ge⟩
-        by simp [← Icc.val_inj, s't]] at memₑ
-      obtain ⟨cap', mem⟩ := qm.mpr ⟨capₑ', memₑ⟩
-      exact ⟨t, ⟨cap', mem⟩, rfl⟩
+theorem matchPartialFree_star_greedy {r : Regex α}
+    (rf : r.MatchPartialFree)
+    : [/⟨r⟩*/].MatchPartialFree := by
+  rw [MatchPartialFree]
+  simp only [matchPartial_star, star_terminates']
+  rw [← MatchPartialFree.eq_1]
+  refine matchPartialFree_or (matchPartialFree_or ?_ ?_) matchPartialFree_empty
+  ·
 
 end MatchPartialShrink
 
